Low/Reduce_by_P_compose.v
@@ -1,20 +1,9 @@
 From Tweetnacl Require Import Libs.Export.
 From Tweetnacl Require Import ListsOp.Export.
-(* From Tweetnacl Require Import Mid.SubList. *)
-(* From Tweetnacl Require Import Low.Get_abcdef. *)
-(* From Tweetnacl Require Import Low.GetBit_pack25519. *)
-(* From Tweetnacl Require Import Low.Sel25519. *)
-(* From Tweetnacl Require Import Low.Constant. *)
-(* From Tweetnacl Require Import Libs.Lists_extended.
-From Tweetnacl Require Import Libs.List_Ltac.
-From Tweetnacl Require Import Libs.LibTactics_SF.
-From Tweetnacl Require Import Libs.LibTactics.
-From Tweetnacl Require Import Libs.LibTactics.
- *)
 From Tweetnacl Require Import Low.Reduce_by_P_compose_step.
 From Tweetnacl Require Import Low.Reduce_by_P_compose_1.
 From Tweetnacl Require Import Low.Reduce_by_P_compose_2.
-From stdpp Require Import prelude.
+Require Import ssreflect.
 Require Import Recdef.
 
 (*
@@ -63,53 +52,287 @@ Open Scope Z.
  *   DEFINE SEMANTIC
  *)
 
+Section red_expr.
+
+Instance  term_dec : Decidable := 
+{
+  decide := term_decide;
+  denote := term_denote;
+  decide_impl := term_decide_impl
+}.
+
 Inductive red_expr :=
   | R_red : term -> red_expr
   | Sub_red : red_expr -> red_expr
   | SubC_red : red_expr -> red_expr -> red_expr
-  | Mod_red : red_expr -> red_expr.
+  | Mod_red : red_expr -> red_expr
+  | Nth_red : nat -> list red_expr -> red_expr -> red_expr.
 
-Inductive formula_red_expr := 
-  | Eq_red : list red_expr -> list red_expr -> formula_red_expr.
+(* forall (A : Type) (P : list A -> Prop),
+       P nil -> (forall (a : A) (l : list A), P l -> P (a :: l)) -> forall l : list A, P l *)
+Lemma red_expr_indp : forall (P : red_expr -> Prop),
+       (forall t, P (R_red t)) ->
+       (forall t, P t -> P (Sub_red t)) ->
+       (forall t t', P t -> P t' -> P (SubC_red t t')) ->
+       (forall t, P t -> P (Mod_red t)) ->
+       (forall l n v, P v -> (forall q, In q l -> P q) ->  P (Nth_red n l v)) ->
+       forall l, P l.
+Proof.
+intros P HR HS HC HM HN.
+fix 1.
+destruct l ;
+first [
+   apply HR 
+  | apply HS
+  | apply HC
+  | apply HM
+  | apply HN] ; try apply red_expr_indp.
+induction l ; intros. inversion H.
+simpl in H ; destruct H.
+rewrite <- H.
+apply red_expr_indp.
+apply IHl.
+apply H.
+Qed.
 
 Fixpoint red_expr_denote env (m : red_expr) : Z :=
   match m with
-  | R_red  v  => term_denote env v
+  | R_red  v  => denote env v
   | Sub_red x => subst_0xffff (red_expr_denote env x)
   | SubC_red x y => subst_c (red_expr_denote env x) (red_expr_denote env y)
   | Mod_red x => mod0xffff (red_expr_denote env x)
+  | Nth_red n x v => nth n  (map (red_expr_denote env) x) (red_expr_denote env v)
   end.
 
+Fixpoint red_expr_simplify (l1:red_expr) :red_expr := match  l1 with
+  | Nth_red n x v => nth_f red_expr_simplify v n x
+  | _ => l1
+end.
+
+Lemma red_expr_simplify_denote : forall env l, red_expr_denote env (red_expr_simplify l) = red_expr_denote env l.
+Proof.
+intros env.
+induction l using red_expr_indp ; try reflexivity.
+simpl.
+rewrite -nth_f_ext map_nth.
+destruct (nth_in_or_default n l l0) as [Hi|Hv].
+apply H in Hi; assumption.
+rewrite Hv; apply IHl.
+Qed.
+
+
+Fixpoint red_expr_decide_rec (l1 l2:red_expr) := match l1, l2 with
+  | R_red v1 , R_red v2 => decide v1 v2
+  | Sub_red v1, Sub_red v'1 => (red_expr_decide_rec v1 v'1)
+  | SubC_red v1 v2, SubC_red v'1 v'2 => andb (red_expr_decide_rec v1 v'1) (red_expr_decide_rec v2 v'2)
+  | Mod_red v1, Mod_red v2 => red_expr_decide_rec v1 v2
+  | _, _ => false
+  end.
+
+Definition red_expr_decide (l1 l2:red_expr) := red_expr_decide_rec (red_expr_simplify l1) (red_expr_simplify l2).
+Transparent red_expr_decide.
+
+Lemma red_expr_decide_trans : forall l l', red_expr_decide_rec l l' = true -> red_expr_decide l l' = true.
+Proof.
+intros.
+destruct l, l' ; try assumption ; simpl in H ; discriminate.
+Qed.
+
+(* Fixpoint red_expr_decide (l1 l2:red_expr) := match (red_expr_simplify l1), (red_expr_simplify l2) with
+  | R_red v1 , R_red v2 => decide v1 v2
+  | Sub_red v1, Sub_red v'1 => (red_expr_decide v1 v'1)
+  | SubC_red v1 v2, SubC_red v'1 v'2 => andb (red_expr_decide v1 v'1) (red_expr_decide v2 v'2)
+  | Mod_red v1, Mod_red v2 => red_expr_decide v1 v2
+  | _, _ => false
+  end.
+ *)
+
+Lemma red_expr_decide_impl:
+  forall env l l', 
+  red_expr_decide l l' = true ->
+  red_expr_denote env l = red_expr_denote env l'.
+Proof.
+intros env.
+induction l using red_expr_indp.
+(* case R_red *)
+intros.
+destruct l'; simpl in H ; try discriminate.
+cbn in H ; apply term_decide_impl ; assumption.
+cbn in H.
+cbn.
+rewrite map_nth.
+
+rewrite -nth_f_ext in H.
+destruct (nth_in_or_default n l l') as [H'|H'].
+destruct (red_expr_simplify (nth n l l')) eqn:? ; try  discriminate.
+rewrite -red_expr_simplify_denote Heqr ; simpl.
+apply term_decide_impl ; assumption.
+
+rewrite H'.
+rewrite H' in H.
+destruct (red_expr_simplify l') eqn:? ; try  discriminate.
+rewrite -red_expr_simplify_denote Heqr ; simpl.
+apply term_decide_impl ; assumption.
+
+(* case Sub_red *)
+intros.
+destruct l' ; simpl in H ; try discriminate.
+cbn in H ; cbn;
+apply red_expr_decide_trans in H;
+apply IHl in H ; f_equal ; assumption.
+
+cbn in H; rewrite -nth_f_ext in H.
+destruct (nth_in_or_default n l0 l') as [H'|H'].
+destruct (red_expr_simplify (nth n l0 l')) eqn:? ; try discriminate;
+simpl; rewrite map_nth; symmetry ; rewrite -red_expr_simplify_denote Heqr ; symmetry; simpl;
+apply red_expr_decide_trans in H;
+f_equal; apply IHl ; assumption.
+
+rewrite H' in H.
+destruct (red_expr_simplify l') eqn:? ; try discriminate.
+simpl; rewrite map_nth; symmetry. rewrite -red_expr_simplify_denote H' Heqr ; symmetry; simpl;
+apply red_expr_decide_trans in H;
+f_equal; apply IHl ; assumption.
+
+(* case SubC_red *)
+intros.
+destruct l' ; simpl in H ; try discriminate.
+cbn in H ; cbn.
+destruct (andb_prop _ _ H)  as [H' H''].
+apply red_expr_decide_trans in H'.
+apply red_expr_decide_trans in H''.
+apply IHl1 in H';
+apply IHl2 in H''.
+rewrite H' H''.
+reflexivity.
+
+cbn in H.
+cbn.
+rewrite map_nth.
+
+rewrite -nth_f_ext in H.
+destruct (nth_in_or_default n l l') as [H3|H3].
+destruct (nth n l l') eqn:? ; simpl in * ; try discriminate.
+destruct (andb_prop _ _ H)  as [H' H''].
+apply red_expr_decide_trans in H'.
+apply red_expr_decide_trans in H''.
+apply IHl1 in H';
+apply IHl2 in H''.
+rewrite H' H''.
+reflexivity.
+
+rewrite -nth_f_ext in H;
+destruct (red_expr_simplify (nth n0 l0 r)) eqn:? => //= .
+rewrite map_nth ; simpl ; symmetry ; rewrite -red_expr_simplify_denote Heqr0.
+destruct (andb_prop _ _ H)  as [H' H''].
+apply red_expr_decide_trans in H'.
+apply red_expr_decide_trans in H''.
+apply IHl1 in H';
+apply IHl2 in H''.
+rewrite H' H''.
+reflexivity.
+
+rewrite H3.
+rewrite H3 in H.
+destruct (red_expr_simplify l') eqn:?  => //=;
+symmetry;
+rewrite -red_expr_simplify_denote Heqr ; simpl.
+destruct (andb_prop _ _ H)  as [H' H''].
+apply red_expr_decide_trans in H'.
+apply red_expr_decide_trans in H''.
+apply IHl1 in H';
+apply IHl2 in H''.
+rewrite H' H''.
+reflexivity.
+
+(* case Mod_red *)
+intros.
+destruct l' ; simpl in H ; try discriminate.
+cbn in H ; cbn;
+apply red_expr_decide_trans in H;
+apply IHl in H ; f_equal ; assumption.
+
+cbn in H; rewrite -nth_f_ext in H.
+destruct (nth_in_or_default n l0 l') as [H'|H'].
+destruct (red_expr_simplify (nth n l0 l')) eqn:? ; try discriminate;
+simpl; rewrite map_nth; symmetry ; rewrite -red_expr_simplify_denote Heqr ; symmetry; simpl;
+apply red_expr_decide_trans in H;
+f_equal; apply IHl ; assumption.
+
+rewrite H' in H.
+destruct (red_expr_simplify l') eqn:? ; try discriminate.
+simpl; rewrite map_nth; symmetry. rewrite -red_expr_simplify_denote H' Heqr ; symmetry; simpl;
+apply red_expr_decide_trans in H;
+f_equal; apply IHl ; assumption.
+
+(* case Nth_red *)
+
+intros l' H'.
+simpl.
+rewrite map_nth.
+destruct (nth_in_or_default n l l0) as [H''|H''].
+apply H ; try assumption.
+cbn in H' ; rewrite -nth_f_ext in H'; assumption.
+
+rewrite H''.
+apply IHl.
+cbn in H'.
+rewrite -nth_f_ext in H'.
+rewrite H'' in H'.
+assumption.
+Qed.
+
+End red_expr.
+
+Instance  red_expr_dec : Decidable := 
+{
+  decide := red_expr_decide;
+  denote := red_expr_denote;
+  decide_impl := red_expr_decide_impl
+}.
+
+(*
 Fixpoint red_expr_list_denote env (m: list red_expr) : list Z :=
   match m with
   | nil => nil
   | h :: q => (red_expr_denote env h) :: red_expr_list_denote env q
   end.
+*)
 
+(*
 Lemma red_expr_list_denote_nth :
   forall i env l, red_expr_denote env (nth i l (R_red (Val 0))) = nth i (red_expr_list_denote env l) 0.
 Proof.
 intros i env l. gen i. induction l as [|h l IHl] ; intros [|i] ; try reflexivity.
 simpl. apply IHl.
 Qed.
-
+*)
+(* 
 Lemma red_expr_list_denote_upd_nth :
   forall i env l v, red_expr_list_denote env (upd_nth i l v) = upd_nth i (red_expr_list_denote env l) (red_expr_denote env v).
 Proof.
 intros i env m. gen i. induction m as [|h m IHm] ; intros [|i] v ; try reflexivity.
 simpl. f_equal. apply IHm.
 Qed.
-
-Definition formula_red_expr_denote env (t : formula_red_expr) : Prop :=
+ *)
+(* Definition formula_red_expr_denote env (t : formula_red_expr) : Prop :=
   match t with
   | Eq_red x y     => red_expr_list_denote env x = red_expr_list_denote env y
   end.
 
+ *)
 (*****************************************************************************************
  *   DECIDE EQUALITY
  *)
 
-Fixpoint decide_red_expr_eq (l1 l2:red_expr) := match l1, l2 with
+(* Scheme Equality for red_expr. *)
+(* Print term_beq. *)
+(* Scheme Equality for list. *)
+
+(* Print red_expr_beq. *)
+(* Print list_beq. *)
+
+(* Fixpoint red_expr_decide (l1 l2:red_expr) := match l1, l2 with
   | R_red v1 , R_red v2 => term_eqb v1 v2
   | Sub_red v1, Sub_red v'1 => (decide_red_expr_eq v1 v'1)
   | SubC_red v1 v2, SubC_red v'1 v'2 => andb (decide_red_expr_eq v1 v'1) (decide_red_expr_eq v2 v'2)
@@ -123,24 +346,9 @@ Fixpoint decide_red_expr_list_eq (l1 l2:list red_expr) := match l1, l2 with
   | _, _ => false
 end.
 
-Lemma decide_red_expr_eq_impl:
-  forall env l l', 
-  decide_red_expr_eq l l' = true ->
-  red_expr_denote env l = red_expr_denote env l'.
-Proof.
-intros env.
-induction l; intros [] H ; simpl in * ;
-repeat match goal with
-  | _ => discriminate
-  | _ => reflexivity
-  | [ H : _ && _ = true |- _ ] => apply andb_prop in H; destruct H
-  | [ H : term_eqb _ _ = true |- _ ] => apply term_eqb_refl in H; subst
-  | [ H : _ = _ |- _ ] => rewrite H
-  | [ H : _ , H1 : _ |- _ ] => apply H in H1 (* why bother ? :D *)
-end.
-Qed.
+ *)
 
-Lemma decide_red_expr_list_eq_impl:
+(* Lemma decide_red_expr_list_eq_impl:
   forall env l l',
   decide_red_expr_list_eq l l' = true ->
   red_expr_list_denote env l = red_expr_list_denote env l'.
@@ -156,16 +364,23 @@ repeat match goal with
   | [ H : _ = _ |- _ ] => rewrite H
   | [ H : False |- _ ] => destruct H
 end.
-Qed.
+Qed. *)
 
-Definition decide_formula_red_expr (f : formula_red_expr) : bool := match f with
+(* Definition decide_formula_red_expr (f : formula_red_expr) : bool := match f with
   | Eq_red x y => decide_red_expr_list_eq x y
   end.
-
-Lemma decide_formula_red_impl : forall env f, decide_formula_red_expr f = true -> formula_red_expr_denote env f.
+ *)
+(* Lemma decide_formula_red_impl : forall env f, decide_formula_red_expr f = true -> formula_red_expr_denote env f.
 Proof. intros env [? ?]. by apply decide_red_expr_list_eq_impl. Qed.
-
+ *)
 (* Weaponize our expression so we can translate functions *)
+
+Instance list_red_expr : Decidable :=
+{
+  decide := list_upd_ext_decide red_expr_dec;
+  denote := list_upd_ext_denote red_expr_dec;
+  decide_impl := list_upd_ext_decide_impl red_expr_dec
+}.
 
 Definition sub_red_step (a:Z) (m t:list red_expr) : list red_expr :=
     let m' := nth (Z.to_nat (a - 1)) m (R_red (Val 0)) in
@@ -176,10 +391,11 @@ Definition sub_red_step_1 (a:Z) (m t:list red_expr) : list red_expr :=
     let t' := nth (Z.to_nat a) t (R_red (Val 0)) in
       (upd_nth (Z.to_nat a) m (Sub_red t')).
 
-Definition sub_red_step_2 (a:Z) (m:list red_expr) : list red_expr :=
-    let m' := nth (Z.to_nat (a - 1)) m (R_red (Val 0)) in
-    let t' := nth (Z.to_nat a) m (R_red (Val 0)) in
-      upd_nth (Z.to_nat (a-1)) (upd_nth (Z.to_nat a) m (SubC_red t' m')) (Mod_red m').
+Definition sub_red_step_2 (a:Z) (m:list red_expr) : @list_upd_ext red_expr :=
+    let m' := Nth_red (Z.to_nat (a - 1)) m (R_red (Val 0)) in
+    let t' := Nth_red (Z.to_nat a) m (R_red (Val 0)) in
+      Upd (Z.to_nat (a-1)) (Upd (Z.to_nat a) m (SubC_red t' m')) (Mod_red m').
+
 
 Lemma step_fn_red_expr : forall env a m t,
   sub_fn_rev sub_step a (red_expr_list_denote env m) (red_expr_list_denote env t) =
@@ -222,13 +438,31 @@ Lemma step_fn_red_expr_1 : forall env a m t,
 Proof.
 intros env [ | p | p] m t.
 all: try reflexivity.
+(* pattern p. *)
+(* induction p using Pos.peano_ind. *)
 assert(Hi:= Pos2Z.is_nonneg p).
 remember (Z.pos p) as i.
 clears p.
 gen m t.
+(* Check nat_ind.
+About natlike_ind.
+Locate natlike_ind.
+SearchAbout positive "peano".
+Axiom natlike_ind' : forall P : forall (z : Z) (pf : 0 <= z), Prop, (forall pf, P 0 pf) -> (forall z pf pf', P z pf -> P (Z.succ z) pf') -> forall z pf, P z pf.
+induction i,Hi using natlike_ind'.
+induction i,Hi using natlike_ind.
+induction Hi,i using natlike_ind. *)
+(* gen Hi. *)
+pattern i.
+apply natlike_ind ;try omega.
+(* match goal with 
+  | [ |- ?f p ] => apply (natlike_ind f)
+end.
+
 apply (natlike_ind (fun i => ∀ m t : list red_expr,
 sub_fn_rev sub_step_1 i (red_expr_list_denote env m) (red_expr_list_denote env t) =
 red_expr_list_denote env (sub_fn_rev sub_red_step_1 i m t))) ; try omega.
+ *)
 intros ; reflexivity.
 clears i.
 intros i Hi IH m t.
