Libs/Decidable.v
@@ -1,0 +1,15 @@
+Require Export Coq.ZArith.ZArith.
+
+Record environment := { vars : positive -> Z }.
+
+Open Scope Z_scope.
+
+Class Decidable {T U: Type} :=
+  {
+    decide : T -> T -> bool;
+    denote : environment -> T -> U;
+    decide_impl: forall (env:environment) (a b :T),
+      decide a b = true -> denote env a = denote env b
+  }.
+
+Close Scope Z.
