Libs/Expr_Decidable.v
@@ -1,0 +1,340 @@
+Set Warnings "-notation-overridden".
+
+Require Export Coq.ZArith.ZArith.
+Require Export Coq.Lists.List.
+Require Import Coq.Sorting.Sorting Orders.
+Require Import ssreflect.
+Require Import Tweetnacl.Libs.Decidable.
+Require Import Tweetnacl.Libs.Term_Decidable.
+
+Open Scope Z_scope.
+(*
+Instance term_dec : Decidable := 
+{
+  decide := term_eqb;
+  denote := term_denote;
+  decide_impl := term_eqb_impl
+}.
+ *)
+
+Module TermOrder <: TotalLeBool.
+    Definition t := term.
+    Definition leb x y := term_leb x y.
+
+    Theorem leb_total : forall a1 a2, leb a1 a2 = true \/ leb a2 a1 = true.
+    Proof.
+      move=> a b.
+      unfold leb, term_leb.
+      destruct a, b.
+      rewrite !Pos2Z.inj_leb.
+      assert(H:= Zle_bool_total (Z.pos p) (Z.pos p0)).
+      destruct H as [H|H] ; rewrite H ; auto.
+      by right.
+      by left.
+      assert(H:= Zle_bool_total z z0).
+      destruct H as [H|H] ; rewrite H ; auto.
+    Qed.
+End TermOrder.
+
+Module ListTermOrder <: TotalLeBool.
+  Definition t := list term.
+
+  Fixpoint leb x y := match x, y with
+    | nil , _ => true
+    | _ , nil => false
+    | a :: qa, b :: qb => match term_ltb a b with
+      | true => true
+      | false => match term_decide a b with
+        | true => leb qa qb
+        | false => false
+        end
+      end
+  end.
+
+  Theorem leb_total : forall a1 a2, leb a1 a2 = true \/ leb a2 a1 = true.
+  Proof.
+  elim => [| a qa IHa].
+  by left.
+  move=> [| b qb] ; simpl.
+  by right.
+  specialize IHa with qb ; simpl.
+  destruct(term_ltb a b) eqn:H0 ; destruct(term_ltb b a) eqn:H1.
+  by left.
+  by left.
+  by right.
+  destruct(term_decide a b) eqn:H2; destruct(term_decide b a) eqn:H3.
+  auto.
+  move: H3 ; rewrite term_decide_com; congruence.
+  move: H3 ; rewrite term_decide_com; congruence.
+  exfalso.
+  clear IHa.
+  unfold term_ltb, term_decide in *.
+  destruct a, b ; try discriminate.
+  move: H2 ; rewrite Pos2Z.inj_eqb Z.eqb_neq.
+  move: H0 ; rewrite Pos2Z.inj_ltb Z.ltb_ge.
+  move: H1 ; rewrite Pos2Z.inj_ltb Z.ltb_ge.
+  move => ? ? ?.
+  omega.
+  move: H2 ; rewrite Z.eqb_neq.
+  move: H0 ; rewrite Z.ltb_ge.
+  move: H1 ; rewrite Z.ltb_ge.
+  move => ? ? ?.
+  omega.
+  Qed.
+End ListTermOrder.
+
+Module Import TermSort := Sort TermOrder.
+Module Import ListTermSort := Sort ListTermOrder.
+
+Section Expr.
+  Inductive expr :=
+    | R : term -> expr
+    | A : expr -> expr -> expr
+    | M : term -> term -> expr.
+
+  Fixpoint expr_denote (env:environment) (m : expr) : Z :=
+    match m with
+    | R v   => denote env v
+    | A x y => expr_denote env x + expr_denote env y
+    | M x y => denote env x * denote env y
+    end.
+
+  Fixpoint latten_expr (e : expr) : (list (list term)) := match e with
+    | A a b => latten_expr a ++ latten_expr b
+    | M a b => (a :: b :: nil) :: nil
+    | R x => (x :: nil) :: nil
+  end.
+
+  Fixpoint simplify_M (l: list term) : list term := match l with
+    | nil => nil
+    | Val 1 :: q => simplify_M q
+    | h :: q => h :: simplify_M q
+    end.
+
+  Fixpoint ldenote_M (env:environment) (ls : list term) : Z :=
+    match ls with
+      | nil => 1
+      | x :: ls' => denote env x * (ldenote_M env ls')
+    end.
+
+  Local Lemma ldenote_M_cons: forall (env:environment) a l, ldenote_M env (a::l) =  (denote env a) * ldenote_M env l.
+  Proof. by move=> //. Qed.
+
+  Local Lemma ldenote_M_app: forall (env:environment) a b, ldenote_M env (a ++ b) = ldenote_M env a * ldenote_M env b.
+  Proof. induction a ; intros ; simpl => //.
+  destruct (ldenote_M env b) ; auto.
+  rewrite IHa ; ring.
+  Qed.
+
+  Local Lemma ldenote_M_simplify: forall (env:environment)  l, ldenote_M env l = ldenote_M env (simplify_M l).
+  Proof. induction l as [|h l IHl] => //=.
+  rewrite IHl. destruct h. by destruct p.
+  destruct z ; try destruct p ; try reflexivity.
+  simpl term_denote. ring.
+  Qed.
+
+  Local Lemma simplifiy_M_0 : forall (env:environment) a, existsb (decide (Val 0)) a = true -> ldenote_M env a = 0.
+  Proof.
+  induction a => //=.
+  rewrite Bool.orb_true_iff => H.
+  case H ; clear H => H.
+  destruct a ; try discriminate.
+  destruct z ; try discriminate.
+  simpl term_denote ; omega.
+  apply IHa in H ; rewrite H ; omega.
+  Qed.
+
+  Fixpoint simplify_A (l :list (list term)) : list (list term) := match l with
+    | nil => nil
+    | h :: q => let s := simplify_M h in
+      match existsb (decide (Val 0)) s with
+      | true => simplify_A q
+      | false => s :: simplify_A q
+      end
+    end.
+
+  Fixpoint ldenote (env:environment) (ls : list (list term)) : Z :=
+    match ls with
+      | nil => 0
+      | x :: ls' => (ldenote_M env x) + (ldenote env ls')
+    end.
+
+  Local Lemma ldenote_cons: forall (env:environment) a l, ldenote env (a::l) = (ldenote_M env a) + ldenote env l.
+  Proof. by move=> //. Qed.
+
+  Local Lemma ldenote_app: forall (env:environment) a b, ldenote env (a ++ b) = ldenote env a + ldenote env b.
+  Proof.
+  induction a ; intros ; simpl => //.
+  rewrite IHa ; ring.
+  Qed.
+
+  Local Lemma latten_expr_correct : forall (env:environment)  t, expr_denote env t = ldenote env (latten_expr t).
+  Proof.
+  induction t ; simpl ; try ring.
+  rewrite ldenote_app IHt1 IHt2 => //.
+  Qed.
+
+  Local Lemma ldenote_simplify: forall (env:environment)  l, ldenote env l = ldenote env (simplify_A l).
+  Proof. induction l ; intros ; simpl => //.
+  destruct (existsb (term_decide (Val 0)) (simplify_M a)) eqn:H; auto.
+  apply (simplifiy_M_0 env) in H.
+  move: H ; rewrite -ldenote_M_simplify => -> ; omega.
+  simpl; rewrite -?ldenote_M_simplify; omega.
+  Qed.
+
+  Definition flatten_expr t := simplify_A (latten_expr t).
+
+  Local Lemma flatten_expr_correct : forall (env:environment) t, expr_denote env t = ldenote env (flatten_expr t).
+  Proof. move => env t. unfold flatten_expr.
+  rewrite -ldenote_simplify.
+  apply latten_expr_correct.
+  Qed.
+
+(*****************************************************************************************
+ *   SORT THE LIST
+ *)
+
+
+  Local Lemma perm_ldenote_M : forall (env:environment)  l l', Permutation.Permutation l l' -> ldenote_M env l = ldenote_M env l'.
+  Proof.
+    intros env l l' H.
+    induction H => // ; simpl.
+    by rewrite IHPermutation.
+    ring.
+    by rewrite IHPermutation1 IHPermutation2.
+  Qed.
+
+  Local Lemma sort_ldenote_M : forall (env:environment) l, ldenote_M env l = ldenote_M env (TermSort.sort l).
+  Proof.
+    intros.
+    apply perm_ldenote_M.
+    apply TermSort.Permuted_sort.
+  Qed.
+
+  Definition flatten_eq l := ListTermSort.sort (map TermSort.sort l).
+
+  Local Lemma perm_ldenote : forall (env:environment)  l l', Permutation.Permutation l l' -> ldenote env l = ldenote env l'.
+  Proof.
+    intros env  l l' H.
+    induction H => // ; simpl.
+    by rewrite IHPermutation.
+    ring.
+    by rewrite IHPermutation1 IHPermutation2.
+  Qed.
+
+  Local Lemma sort_ldenote : forall (env:environment)  l, ldenote env l = ldenote env (ListTermSort.sort l).
+  Proof.
+    intros.
+    apply perm_ldenote.
+    apply Permuted_sort.
+  Qed.
+
+  Theorem flatten_eq_denote : forall (env:environment)  l, ldenote env l = ldenote env (flatten_eq l).
+  Proof.
+    induction l => //.
+    unfold flatten_eq in *.
+    rewrite -sort_ldenote.
+    simpl.
+    f_equal.
+    apply sort_ldenote_M.
+    by rewrite -sort_ldenote in IHl.
+  Qed.
+
+(*****************************************************************************************
+ *   DECIDE EQUALITY
+ *)
+
+  Fixpoint decide_list_term_eq (l l':list term): bool := match l, l' with
+    | nil , nil => true
+    | a:: qa , b :: qb => andb (decide a b) (decide_list_term_eq qa qb)
+    | _, _ => false
+    end.
+
+  Local Lemma decide_list_term_eq_impl:
+    forall (env:environment) l l', 
+    decide_list_term_eq l l' = true ->
+    ldenote_M env l = ldenote_M env l'.
+  Proof.
+  induction l ; destruct l' ; auto => H.
+  simpl in H ; discriminate.
+  simpl in H ; discriminate.
+  simpl in *.
+  move: H; rewrite !Bool.andb_true_iff ; move=> [Ht Hl].
+  apply IHl in Hl.
+  f_equal.
+  apply term_decide_impl.
+  all: assumption.
+  Qed.
+
+  Local Fixpoint decide_list_list_term (l l':list (list term)) : bool := match l, l' with
+    | nil, nil => true
+    | a:: qa , b :: qb => andb (decide_list_term_eq a b) (decide_list_list_term qa qb)
+    | _, _ => false
+    end.
+
+  Local Lemma decide_list_list_term_eq_impl : forall (env:environment)  l l', decide_list_list_term l l' = true ->
+    ldenote env l = ldenote env l'.
+  Proof.
+  induction l ; destruct l' ; auto => H.
+  simpl in H ; discriminate.
+  simpl in H ; discriminate.
+  simpl in *.
+  move: H; rewrite !Bool.andb_true_iff ; move=> [Ht Hl].
+  apply IHl in Hl.
+  apply (decide_list_term_eq_impl env) in Ht.
+  rewrite Ht Hl ; reflexivity.
+  Qed.
+
+Definition decide_llt (l l':list (list term)) : bool := decide_list_list_term (flatten_eq l) (flatten_eq l').
+
+Definition expr_decide (e e': expr) : bool := decide_llt (flatten_expr e) (flatten_expr e').
+
+Lemma expr_decide_impl:
+  forall (env:environment) a b,
+    expr_decide a b = true ->
+    expr_denote env a = expr_denote env b.
+Proof.
+  intros env a b Hdec.
+  unfold expr_decide in Hdec.
+  unfold decide_llt in Hdec.
+  assert(H: exists l, l = flatten_expr a).
+    eexists. reflexivity.
+  destruct H as [l Hl].
+  assert(Hld: ldenote env l = expr_denote env a).
+    rewrite flatten_expr_correct; subst => //.
+  assert(H: exists l, l = flatten_expr b).
+    eexists. reflexivity.
+  destruct H as [l' Hl'].
+  assert(Hl'd: ldenote env l' = expr_denote env b).
+    rewrite flatten_expr_correct; subst => //.
+  rewrite -Hld -Hl'd.
+  rewrite flatten_eq_denote ; symmetry ; rewrite flatten_eq_denote ; symmetry ; subst.
+  by apply decide_list_list_term_eq_impl.
+Qed.
+
+End Expr.
+
+Local Definition ta := Var 1%positive.
+Local Definition tb := Var 2%positive.
+Local Definition tc := Var 3%positive.
+Local Definition td := Var 4%positive.
+Local Definition te := Var 5%positive.
+Local Definition tf := Var 6%positive.
+Local Definition tg := Var 7%positive.
+
+Local Definition expr1 := A (M ta tb) (A (R tc) (R tb)).
+Local Definition expr2 := A (A (R tc) (R tb)) (M ta tb).
+(* Eval compute in flatten_expr expr1. *)
+(* Eval compute in flatten_eq (flatten_expr expr1). *)
+(* Eval compute in (flatten_expr expr2). *)
+(* Eval compute in flatten_eq (flatten_expr expr2). *)
+
+
+Instance expr_dec : Decidable := Build_Decidable expr Z expr_decide (expr_denote) expr_decide_impl.
+
+Local Example test1 : expr_decide expr1 expr2 = true.
+Proof.
+by compute.
+Qed.
+
+Close Scope Z.
