Libs/List_ext_Decidable.v
@@ -1,0 +1,136 @@
+Set Warnings "-notation-overridden".
+Require Export Coq.ZArith.ZArith.
+Require Export Coq.Lists.List.
+Require Import Tweetnacl.Libs.Decidable.
+Require Import Tweetnacl.Libs.Expr_Decidable.
+Require Import Tweetnacl.Libs.Term_Decidable.
+Require Import Tweetnacl.Libs.List_Decidable.
+Require Import Tweetnacl.Libs.Lists_extended.
+Require Import ssreflect.
+
+Open Scope Z_scope.
+
+Section list_upd_denote.
+
+Context {T} {U} (inst : @Decidable T U).
+Instance  list_dec : Decidable := 
+{
+  decide := list_decide inst;
+  denote := list_denote inst;
+  decide_impl := list_decide_impl inst
+}.
+
+Inductive list_upd_ext :=
+  | List  : list T -> list_upd_ext
+  | Upd   : nat -> list_upd_ext -> T -> list_upd_ext.
+
+Fixpoint list_upd_ext_denote (env:environment) (l:list_upd_ext) : list U := match l with
+  | List l'    => denote env l'
+  | Upd n l' v => upd_nth n (list_upd_ext_denote env l') (denote env v)
+end.
+
+Local Lemma upd_nth_denote : forall (env:environment) n l v,
+  upd_nth n (list_denote inst env l) (denote env v) = denote env (upd_nth n l v).
+Proof.
+induction n as [|n IHn] ; destruct l as [|h l] => v //.
+simpl. rewrite IHn.
+reflexivity.
+Qed.
+
+Local Lemma upd_nth_list_upd_ext_denote : forall (env:environment) n l v,
+  upd_nth n (list_upd_ext_denote env l) (denote env v) = list_upd_ext_denote env (Upd n l v).
+Proof. reflexivity. Qed.
+
+Fixpoint SomeList (n:nat) (m:list_upd_ext) (v:T) : list T := match m with
+  | List l => upd_nth n l v
+  | Upd n' l' v' => upd_nth n (SomeList n' l' v') v
+end.
+
+Local Lemma SomeListDenote : forall (env:environment) (n:nat) (l:list_upd_ext) (v:T),
+  list_upd_ext_denote env (Upd n l v) = list_upd_ext_denote env (List (SomeList n l v)).
+Proof.
+  intros env.
+  fix 2.
+  intros n l v.
+  destruct l ; simpl; change (list_denote _ ?A ?B) with (denote A B);
+  rewrite -upd_nth_denote ;  try reflexivity.
+  specialize SomeListDenote with n0 l t;
+  simpl in SomeListDenote;
+  rewrite SomeListDenote;
+  reflexivity.
+Qed.
+
+Definition list_upd_ext_decide (l l':list_upd_ext) : bool := match l with
+  | List m         =>
+    match l' with
+      | List m'    => decide m m'
+      | Upd n' m' v' => decide m (SomeList n' m' v')
+    end
+  | Upd n m v     => 
+    match l' with
+      | List m' => decide (SomeList n m v) m'
+      | Upd n' m' v' => decide (SomeList n m v) (SomeList n' m' v')
+    end
+  end.
+
+Lemma list_upd_ext_decide_impl : forall (env:environment) (l l' : list_upd_ext),
+  list_upd_ext_decide l l' = true -> list_upd_ext_denote env l = list_upd_ext_denote env l'.
+Proof.
+  intros env; induction l as [|n l Hl];
+  destruct l' => Hll' ; simpl in *; apply (list_decide_impl inst env) in Hll';
+  repeat change (list_denote inst env ?A) with (list_upd_ext_denote env (List A)) in Hll';
+  change (list_denote inst env ?A) with (list_upd_ext_denote env (List A));
+  rewrite -?SomeListDenote in Hll';
+  assumption.
+Qed.
+
+End list_upd_denote.
+
+(* Section list_nth_denote.
+Context {T} {U} (inst : @Decidable T U).
+Instance  list_dec2 : Decidable := 
+{
+  decide := list_decide inst;
+  denote := list_denote inst;
+  decide_impl := list_decide_impl inst
+}.
+
+Inductive list_nth_ext :=
+  | Nv  : T -> list_nth_ext
+  | Nth : nat -> list T -> T -> list_nth_ext.
+
+Definition list_nth_ext_denote (env:environment) (l:list_nth_ext) : U := match l with
+  | Nv  v    => denote env v
+  | Nth n l' v => nth n (denote env l') (denote env v)
+end.
+
+Local Lemma nth_denote : forall (env:environment) n l v,
+  nth n (list_denote inst env l) (denote env v) = denote env (nth n l v).
+Proof.
+induction n as [|n IHn] ; destruct l as [|h l] => v //.
+simpl. rewrite IHn.
+reflexivity.
+Qed.
+
+Definition list_nth_ext_decide (l l':list_nth_ext) : bool := match l with
+  | Nv m         =>
+    match l' with
+      | Nv m'    => decide m m'
+      | Nth n' m' v' => decide m (nth n' m' v')
+    end
+  | Nth n m v     => 
+    match l' with
+      | Nv m' => decide (nth n m v) m'
+      | Nth n' m' v' => decide (nth n m v) (nth n' m' v')
+    end
+  end.
+
+Lemma list_nth_ext_decide_impl : forall (env:environment) (l l' : list_nth_ext),
+  list_nth_ext_decide l l' = true -> list_nth_ext_denote env l = list_nth_ext_denote env l'.
+Proof.
+  intros env; induction l as [|n l v];
+  destruct l' => Hll' ; simpl in *; rewrite ?nth_denote; by apply decide_impl.
+Qed.
+End list_nth_denote. *)
+
+Close Scope Z.
