Libs/Term_Decidable.v
@@ -1,0 +1,74 @@
+Set Warnings "-notation-overridden".
+
+Require Export Coq.ZArith.ZArith.
+Require Export Coq.Lists.List.
+Require Import Coq.Sorting.Sorting Orders.
+Require Import ssreflect.
+Require Import Tweetnacl.Libs.Decidable.
+
+Open Scope Z_scope.
+
+Inductive term :=
+  | Var   : positive -> term
+  | Val   : Z -> term
+  .
+
+Definition term_decide (x y : term) : bool := match x , y with
+  | Var x , Var y => Pos.eqb x y
+  | Val x,  Val y => Z.eqb x y
+  | _, _ => false
+  end.
+
+Lemma term_eqb_refl : forall x y, term_decide x y = true <-> x = y.
+Proof.
+move => x y ; rewrite /term_decide ; split => H ; simpl.
+destruct x,y; move: H.
+rewrite Pos.eqb_eq => -> //.
+discriminate.
+discriminate.
+rewrite Z.eqb_eq => -> //.
+subst ; destruct y.
+rewrite Pos.eqb_eq //.
+rewrite Z.eqb_eq //.
+Qed.
+
+Definition term_denote (env:environment) (x : term) : Z :=
+  match x with
+  | Var n => vars env n
+  | Val n => n
+  end.
+
+Lemma term_decide_com : forall x y, term_decide x y = term_decide y x.
+Proof.
+move => [] a [] b //=.
+rewrite ?Pos2Z.inj_eqb.
+apply Z.eqb_sym.
+apply Z.eqb_sym.
+Qed.
+
+Definition term_leb (x y : term) : bool := match x , y with
+  | Var x , Var y => Pos.leb x y
+  | Val x , Val y => Z.leb x y
+  | Var x,  Val y => false
+  | Val x,  Var y => true
+  end.
+
+Definition term_ltb (x y : term) : bool := match x , y with
+  | Var x , Var y => Pos.ltb x y
+  | Val x , Val y => Z.ltb x y
+  | Var x,  Val y => false
+  | Val x,  Var y => true
+  end.
+
+Lemma term_decide_impl : forall (env : environment) (a b : term),
+term_decide a b = true -> term_denote env a = term_denote env b.
+Proof. intros. apply term_eqb_refl in H. subst a. reflexivity. Qed.
+
+Instance term_dec : Decidable := 
+{
+  decide := term_decide;
+  denote := term_denote;
+  decide_impl := term_decide_impl
+}.
+
+Close Scope Z.
