Low/Reduce_by_P_compose_1.v
@@ -1,8 +1,8 @@
 From Tweetnacl Require Import Libs.Export.
 From Tweetnacl Require Import ListsOp.Export.
 From Tweetnacl Require Import Low.Reduce_by_P_compose_step.
-
 From stdpp Require Import prelude.
+Require Import ssreflect.
 Require Import Recdef.
 
 Open Scope Z.
@@ -13,6 +13,102 @@ Definition sub_step_1 (a:Z) (m t:list Z) : list Z :=
     let t' := nth (Z.to_nat a) t 0 in
       (upd_nth (Z.to_nat a) m (subst_0xffff t')).
 
+Lemma sub_step_1_Zlength : forall a m t,
+  0 <= a < Zlength m ->
+  Zlength (sub_step_1 a m t) = Zlength m.
+Proof.
+  intros a m t Ham.
+  rewrite /sub_step_1.
+  rewrite ?upd_nth_Zlength.
+  reflexivity.
+  all: rewrite ?Z2Nat.id.
+  all: omega.
+Qed.
 
+Local Lemma sub_fn_rev_s_sub_step_1_ind_Zlength : forall a m t,
+  0 <= a < Zlength m ->
+  Zlength (sub_fn_rev sub_step_1 a m t) = Zlength m ->
+  Zlength (sub_fn_rev sub_step_1 (a+1) m t) = Zlength m.
+Proof.
+  intros i m t Ham Hind.
+  rewrite sub_fn_rev_equation.
+  flatten.
+  replace ( i + 1 - 1) with i by omega.
+  rewrite <- Hind.
+  apply sub_step_1_Zlength.
+  rewrite Hind.
+  assumption.
+Qed.
+
+Lemma sub_fn_rev_s_sub_step_1_Zlength : forall a m t,
+  0 < a < 16 ->
+  Zlength m = 16 ->
+  Zlength (sub_fn_rev sub_step_1 a m t) = Zlength m.
+Proof.
+  intros.
+  pattern a.
+  destruct a.
+  all: try reflexivity.
+  revert H.
+  induction p using Pos.peano_ind.
+  by rewrite sub_fn_rev_1.
+  intros.
+  replace ((Z.pos (Pos.succ p))) with (Z.pos p + 1) by lia.
+  apply sub_fn_rev_s_sub_step_1_ind_Zlength.
+  2: apply IHp.
+  lia.
+  lia.
+Qed.
+
+Local Lemma sub_fn_rev_s_sub_step_1_ind_bound : forall a m t,
+  0 < a < 16 ->
+  Zlength m = 16 ->
+  Forall (fun x => 0 <= x < 2 ^ 16) t ->
+  Forall (fun x => -2^16 + 1 <= x < 1) (take (Z.to_nat a) (sub_fn_rev sub_step_1 a m t)) ->
+  Forall (fun x => -2^16 + 1 <= x < 1) (take (Z.to_nat (a + 1)) (sub_fn_rev sub_step_1 (a + 1) m t)).
+Proof.
+  intros i m t Ham Hm Hbm Hind.
+  rewrite sub_fn_rev_equation.
+  flatten.
+  apply Zle_bool_imp_le in Eq ; omega.
+  replace ( i + 1 - 1) with i by omega.
+  rewrite -(take_cons_Zlength _ _ 0).
+  2: rewrite sub_step_1_Zlength sub_fn_rev_s_sub_step_1_Zlength; omega.
+  remember (sub_fn_rev sub_step_1 i m t) as m'.
+  apply Forall_app_2.
+  rewrite /sub_step_1.
+  rewrite (upd_nth_alter _ (fun x => (subst_0xffff (nth (Z.to_nat i) t 0)))).
+  rewrite take_alter.
+  2: reflexivity.
+  3: reflexivity.
+  assumption.
+  3: apply Forall_cons_2.
+  4: apply Forall_nil ; trivial.
+  3: rewrite /sub_step_1;
+  rewrite upd_nth_same_Zlength /subst_0xffff.
+  3: assert(- 2 ^ 16 + 1 + 65535 ≤ nth (Z.to_nat i) t 0 ∧ nth (Z.to_nat i) t 0 < 1 + 65535) by
+    (change(- 2 ^ 16 + 1 + 65535) with 0 ; change(1 + 65535) with (2^16);
+    apply Forall_nth_d; [compute ; split; go|assumption]).
+  all: try omega.
+  apply Nat2Z.inj_lt.
+  rewrite -Zlength_correct.
+  all: rewrite ?Z2Nat.id ?Heqm' ?sub_fn_rev_s_sub_step_1_Zlength.
+  all: try omega.
+Qed.
+
+Lemma sub_fn_rev_s_sub_step_1_bound : forall i m t,
+  Zlength m = 16 ->
+  0 < i < Zlength m ->
+  Forall (fun x => 0 <= x < 2 ^ 16) t ->
+  Forall (λ a : ℤ, - 2 ^ 16 + 1 ≤ a ∧ a < 1) (take (Z.to_nat 1) m) ->
+  Forall (fun x => -2^16 + 1 <= x < 1) (take (Z.to_nat i) (sub_fn_rev sub_step_1 i m t)).
+Proof.
+intros.
+change(Forall (fun x => -2^16 + 1 <= x < 1) (take (Z.to_nat i) (sub_fn_rev sub_step_1 i m t))) with
+  ((fun x => Forall (fun a => -2^16 + 1 <= a < 1) (take (Z.to_nat x) (sub_fn_rev sub_step_1 x m t))) i).
+apply P016_impl ; try omega.
+rewrite sub_fn_rev_1; assumption.
+intros ; apply sub_fn_rev_s_sub_step_1_ind_bound ; try omega ; try assumption.
+Qed.
 
 Close Scope Z.
