Low/Reduce_by_P_compose_2.v
@@ -1,18 +1,7 @@
 From Tweetnacl Require Import Libs.Export.
 From Tweetnacl Require Import ListsOp.Export.
 From Tweetnacl Require Import Low.Reduce_by_P_compose_step.
-
-(* From Tweetnacl Require Import Mid.SubList. *)
-(* From Tweetnacl Require Import Low.Get_abcdef. *)
-(* From Tweetnacl Require Import Low.GetBit_pack25519. *)
-(* From Tweetnacl Require Import Low.Sel25519. *)
-(* From Tweetnacl Require Import Low.Constant. *)
-(* From Tweetnacl Require Import Libs.Lists_extended.
-From Tweetnacl Require Import Libs.List_Ltac.
-From Tweetnacl Require Import Libs.LibTactics_SF.
-From Tweetnacl Require Import Libs.LibTactics.
- *)
- From stdpp Require Import prelude.
+From stdpp Require Import prelude.
 Require Import Recdef.
 Require Import ssreflect.
 Open Scope Z.
@@ -24,9 +13,51 @@ Definition sub_step_2 (a:Z) (m:list Z) : list Z :=
     let t' := nth (Z.to_nat a) m 0 in
       upd_nth (Z.to_nat (a-1)) (upd_nth (Z.to_nat a) m (subst_c t' m')) (mod0xffff m').
 
+Lemma sub_step_2_Zlength : forall a m,
+  0 < a < Zlength m ->
+  Zlength (sub_step_2 a m) = Zlength m.
+Proof.
+  intros a m Ham.
+  rewrite /sub_step_2.
+  rewrite ?upd_nth_Zlength.
+  reflexivity.
+  all: rewrite ?Z2Nat.id.
+  all: omega.
+Qed.
+
+Lemma sub_fn_rev_s_sub_step_2_ind_Zlength : forall a m,
+  0 < a < Zlength m ->
+  Zlength (sub_fn_rev_s sub_step_2 a m) = Zlength m ->
+  Zlength (sub_fn_rev_s sub_step_2 (a+1) m) = Zlength m.
+Proof.
+  intros i m Ham Hind.
+  rewrite sub_fn_rev_s_equation.
+  flatten.
+  replace ( i + 1 - 1) with i by omega.
+  rewrite <- Hind.
+  apply sub_step_2_Zlength.
+  rewrite Hind.
+  assumption.
+Qed.
+
+Lemma sub_fn_rev_s_sub_step_2_Zlength : forall a m,
+  0 < a < 16 ->
+  Zlength m = 16 ->
+  Zlength (sub_fn_rev_s sub_step_2 a m) = Zlength m.
+Proof.
+  intros.
+  pattern a.
+  apply P016_impl.
+  by rewrite sub_fn_rev_s_1.
+  intros ; apply sub_fn_rev_s_sub_step_2_ind_Zlength.
+  2: apply H2.
+  all: omega.
+Qed.
+
 Lemma sub_step_2_Z_inv : forall a m,
 0 < a < Zlength m ->
 - 2^16 <= nth (Z.to_nat (a - 1)) m 0 <= 0 ->
+(* nth (Z.to_nat (a - 1)) m 0 <= 0 -> *)
 ZofList 16 (sub_step_2 a m) = ZofList 16 m.
 Proof.
 intros a m Hm Hbm.
@@ -53,26 +84,17 @@ rewrite upd_nth_diff_Zlength.
 2,3: rewrite Z2Nat.id.
 all: try omega.
 2: intro H; apply (f_equal Z.of_nat) in H; rewrite ?Z2Nat.id in H; omega.
-replace (2 ^ 16 * (- nth (Z.to_nat a) m 0 + (nth (Z.to_nat a) m 0 - Z.land (nth (Z.to_nat (a - 1)) m 0 ≫ 16) 1)) + (- nth (Z.to_nat (a - 1)) m 0 + Z.land (nth (Z.to_nat (a - 1)) m 0) 65535)) with 
-(2^16 * (nth (Z.to_nat a) m 0) - 2^16 * (nth (Z.to_nat a) m 0) - 2^16 * (Z.land (nth (Z.to_nat (a - 1)) m 0 ≫ 16) 1) + Z.land (nth (Z.to_nat (a - 1)) m 0) 65535 - nth (Z.to_nat (a - 1)) m 0).
-2: ring.
-replace (2 ^ 16 * nth (Z.to_nat a) m 0 - 2 ^ 16 * nth (Z.to_nat a) m 0) with 0 by omega.
 change 65535 with (Z.ones 16).
-change 1 with (Z.ones 1).
-rewrite ?Z.land_ones.
-change (Z.ones 1) with 1.
-2,3: omega.
-match goal with
-| [ |- ?A = _ ] => replace A with (nth (Z.to_nat (a - 1)) m 0 `mod` 2 ^ 16 - (2 ^ 16 * (nth (Z.to_nat (a - 1)) m 0 ≫ 16) `mod` 2 ^ 1 + nth (Z.to_nat (a - 1)) m 0))
+remember (nth _ _ _) as n ; clear Hm Heqn ; clears.
+ring_simplify.
+repeat match goal with
+  | [ |- context[Z.land ?A 1]] => change (Z.land A 1) with (Z.land A (Z.ones 1))
+  | _ => rewrite Z.land_ones
+  | [ |- ?A - _ + _ - _ = _ ] => replace A with 0 by omega
+  | _ => omega
 end.
-2: omega.
-symmetry.
-apply Zplus_minus_eq.
-rewrite -Zplus_0_r_reverse.
-rewrite Zmod_eq.
+rewrite (Zmod_eq _ (2^16)).
 2: apply pown0 ; omega.
-remember (nth (Z.to_nat (a - 1)) m 0) as n.
-clear Hm Heqn ; clears.
 rewrite Z.shiftr_div_pow2.
 2: omega.
 assert(Hn: n = 0 \/ n < 0) by omega.
@@ -90,6 +112,73 @@ rewrite H0.
 change ((-1) `mod` 2 ^ 1 ) with 1.
 ring.
 Qed.
+
+Lemma sub_step_2_Z_bound_nth : forall a m,
+0 < a < Zlength m ->
+- 2^16 < nth (Z.to_nat a) m 0 <= 0 ->
+- 2^16 <= nth (Z.to_nat a) (sub_step_2 a m) 0 <= 0.
+Proof.
+intros a m Hm Hbm.
+rewrite /sub_step_2 /mod0xffff /subst_c.
+rewrite upd_nth_diff_Zlength ?upd_nth_same_Zlength ?upd_nth_Zlength.
+all: try (intro H; apply (f_equal Z.of_nat) in H; rewrite ?Z2Nat.id in H).
+all: rewrite ?Z2Nat.id.
+assert(Hand: Z.land (nth (Z.to_nat (a - 1)) m 0 ≫ 16) 1 = 0 \/ Z.land (nth (Z.to_nat (a - 1)) m 0 ≫ 16) 1 = 1).
+  assert(H:= and_0_or_1 (nth (Z.to_nat (a - 1)) m 0 ≫ 16)) ; omega.
+destruct Hand as [Hand|Hand] ; rewrite Hand.
+all: try omega.
+Qed.
+
+Lemma sub_fn_rev_s_sub_step_2_ind_bound : forall a m,
+  0 < a < 16 ->
+  Zlength m = 16 ->
+  Forall (fun x => 0 <= x < 2^16) m ->
+  Forall (fun x => 0 <= x < 2^16) (take (Z.to_nat a - 1) (sub_fn_rev_s sub_step_2 a m)) ->
+  Forall (fun x => 0 <= x < 2^16) (take (Z.to_nat a) (sub_fn_rev_s sub_step_2 (a + 1) m)).
+Proof.
+Admitted.
+(*   intros i m Ham Hm.
+  rewrite sub_fn_rev_equation.
+  flatten.
+  apply Zle_bool_imp_le in Eq ; omega.
+  replace ( i + 1 - 1) with i by omega.
+  rewrite -(take_cons_Zlength _ _ 0).
+  2: rewrite sub_step_1_Zlength sub_fn_rev_s_sub_step_1_Zlength; omega.
+  remember (sub_fn_rev sub_step_1 i m t) as m'.
+  apply Forall_app_2.
+  rewrite /sub_step_1.
+  rewrite (upd_nth_alter _ (fun x => (subst_0xffff (nth (Z.to_nat i) t 0)))).
+  rewrite take_alter.
+  2: reflexivity.
+  3: reflexivity.
+  assumption.
+  3: apply Forall_cons_2.
+  4: apply Forall_nil ; trivial.
+  3: rewrite /sub_step_1;
+  rewrite upd_nth_same_Zlength /subst_0xffff.
+  3: assert(- 2 ^ 16 + 1 + 65535 ≤ nth (Z.to_nat i) t 0 ∧ nth (Z.to_nat i) t 0 < 1 + 65535) by
+    (change(- 2 ^ 16 + 1 + 65535) with 0 ; change(1 + 65535) with (2^16);
+    apply Forall_nth_d; [compute ; split; go|assumption]).
+  all: try omega.
+  apply Nat2Z.inj_lt.
+  rewrite -Zlength_correct.
+  all: rewrite ?Z2Nat.id ?Heqm' ?sub_fn_rev_s_sub_step_1_Zlength.
+  all: try omega.
+Qed. *)
+
+(* Lemma sub_fn_rev_s_sub_step_1_bound : forall i m t,
+  Zlength m = 16 ->
+  0 < i < Zlength m ->
+  Forall (fun x => 0 <= x < 2 ^ 16) t ->
+  Forall (λ a : ℤ, - 2 ^ 16 + 1 ≤ a ∧ a < 1) (take (Z.to_nat 1) m) ->
+  Forall (fun x => -2^16 + 1 <= x < 1) (take (Z.to_nat i) (sub_fn_rev sub_step_1 i m t)).
+ *)
+
+
+
+Print sub_fn_rev_s.
+Check sub_fn_rev_s_equation.
+Print sub_step_2.
 
 Lemma sub_fn_rev_s_sub_step_2_inv : forall a m,
   0 < a < 16 ->
